---
title: "Equations for models"
author: "Lucas Nell"
date: "11/10/2017"
output:
  pdf_document:
    toc: true
    toc_depth: 2
---

```{r setup, include=FALSE}
knitr::opts_chunk$set(echo = TRUE)
```


This document outlines the equations for models A and B.
Simply knit this `.Rmd` document to get a pdf with rendered equations.

# Model A

## Solving unknown parameters


$$
\begin{aligned}
s_N &= i_N - a_{NP} N_{eq} P_{eq} (1-P_{eq}/k_P) + (1-l_D) m_D D_{eq} \\
s_D &= (1-l_P) m_P P_{eq} + (1-l_V) m_V V_{eq} + (1-l_H) m_H H_{eq} + 
    (1-l_R) m_R R_{eq} - a_{DV} D_{eq} V_{eq} (1-V_{eq}/k_V) - m_D D_{eq} \\
s_P &= a_{NP} N_{eq} P_{eq} (1-P_{eq}/k_P) -  a_{PH} P_{eq} H_{eq} (1-H_{eq}/k_H) - m_P P_{eq} \\
s_V &= a_{DV} D_{eq} V_{eq} (1-V_{eq}/k_V) - (a_R V_{eq} R_{eq}) (1-R_{eq}/k_R) - m_V V_{eq} \\
s_H &= a_{PH} P_{eq} H_{eq} (1-H_{eq}/k_H) - (a_R H_{eq} R_{eq}) (1-R_{eq}/k_R) - m_H H_{eq} \\
s_R &= (a_R V_{eq} R_{eq} + a_R H_{eq} R_{eq}) (1-R_{eq}/k_R) - m_R R_{eq} \\
\end{aligned}
$$


## Differential equations


$$
\begin{aligned}
N &= i_N - a_{NP} N P (1-P/k_P) + (1-l_D) m_D D \\
D &= (1-l_P) m_P P + (1-l_V) m_V V + (1-l_H) m_H H + (1-l_R) m_R R + (1 - l_M) m_M M - a_{DV} D V (1-V/k_V) - m_D D \\
P &= a_{NP} N P (1-P/k_P) - a_{PH} P H (1-H/k_H) - m_P P \\
V &= a_{DV} D V (1-V/k_V) - (a_R V R) (1-R/k_R) - m_V V \\
H &= a_{PH} P H (1-H/k_H) - (a_R H R) (1-R/k_R) - m_H H \\
R &= (a_R V R + a_R H R + \frac{a_R M R}{2} ) (1-R/k_R) - m_R R \\
M &= i_M - m_M M - (\frac{a_R M R}{2}) (1-R/k_R) \\
\end{aligned}
$$



# Model B

## Solving for unknown parameters


$$
\begin{aligned}
s_N &= i_N - a_{NP} N_{eq} P_{eq} (1-P_{eq}/k_P) + (1-l_D) m_D D_{eq} \\
s_D &= (1-l_P) m_P P_{eq} + (1-l_V) m_V V_{eq} + (1-l_H) m_H H_{eq} + (1-l_R) m_R R_{eq} 
    - \frac{a_{DV} D_{eq} V_{eq}}{1+a_{DV} h_D D_{eq}} - m_D D_{eq} \\
s_P &= a_{NP} N_{eq} P_{eq} (1-P_{eq}/k_P) - \frac{a_{PH} P_{eq} H_{eq}}{1+a_{PH} h_P P_{eq}}
    - m_P P_{eq} \\
s_V &= \frac{a_{DV} D_{eq} V_{eq}}{1+a_{DV} h_D D_{eq}} - 
    \frac{a_R V_{eq} R_{eq}}{1+a_R h_R (V_{eq}+H_{eq})} - m_V V_{eq} \\
s_H &= \frac{a_{PH} P_{eq} H_{eq}}{1+a_{PH} h_P P_{eq}} - 
    \frac{a_R H_{eq} R_{eq}}{1+a_R h_R (V_{eq}+H_{eq})} - m_H H_{eq} \\
s_R &= \frac{a_R V_{eq} R_{eq} + a_R H_{eq} R_{eq}}{1+a_R h_R (V_{eq}+H_{eq})} - m_R R_{eq} \\
\end{aligned}
$$

## Differential equations


$$
\begin{aligned}
N &= i_N - a_{NP} N P (1-P/k_P) + (1-l_D) m_D D \\
D &= (1-l_P) m_P P + (1-l_V) m_V V + (1-l_H) m_H H + (1-l_R) m_R R + (1-l_M) m_M M -
    \frac{a_{DV} D V}{1+a_{DV} h_D D} - m_D D \\
P &= a_{NP} N P (1-P/k_P) - \frac{a_{PH} P H}{1+a_{PH} h_P P} - m_P P \\
V &= \frac{a_{DV} D V}{1+a_{DV} h_D D} - \frac{a_R V R}{1+a_R h_R (V+H+M)} - m_V V \\
H &= \frac{a_{PH} P H}{1+a_{PH} h_P P} - \frac{a_R H R}{1+a_R h_R (V+H+M)} - m_H H \\
R &= \frac{a_R V R + a_R H R + a_R M R}{1+a_R hR (V+H+M)} - mR R \\
M &= i_M - m_M M - \frac{a_R M R}{1+a_R h_R (V+H+M)} \\
\end{aligned}
$$